src/coq/QC/ReprAST.v
@@ -7,24 +7,18 @@
     QuickChick. It may be worthwhile to serialize a counterexample
     into a format that it can be imported into Coq for debugging.
 *)
-From ExtLib Require Import
-     Structures.Monads
-     Structures.Functor
-     Eqv.
 
-From Vellvm Require Import LLVMAst Utilities AstLib Syntax.CFG QC.Utils DynamicTypes.
+From Vellvm Require Import LLVMAst ShowAST Utilities DynamicTypes.
 Require Import Integers Floats.
 
 Require Import List.
 
 Import ListNotations.
-Import MonadNotation.
 
 From Coq Require Import
-     ZArith List String Lia Bool.Bool.
+     ZArith List String Bool.Bool.
 
-From QuickChick Require Import QuickChick.
-Import QcDefaultNotation. Open Scope qc_scope.
+From QuickChick Require Import Show.
 Set Warnings "-extraction-opaque-accessed,-extraction".
 
 (* Class for the Coq representation of a structure. *)
@@ -34,22 +28,26 @@ Class Repr A : Type :=
   }.
 
 Section ReprInstances.
-  Global Instance reprList (A : Type) `{Repr A} : Repr (list A) :=
+  #[global]
+   Instance reprList (A : Type) `{Repr A} : Repr (list A) :=
     {
       repr l := ("[" ++ contents repr l ++ "]")%string
     }.
 
-  Global Instance reprInt : Repr LLVMAst.int :=
+  #[global]
+   Instance reprInt : Repr LLVMAst.int :=
     {
       repr i := ("(" ++ show i ++ ")%Z")%string
     }.
 
-  Global Instance reprBool : Repr bool :=
+  #[global]
+   Instance reprBool : Repr bool :=
     {
       repr := show
     }.
 
-  Global Instance reprString : Repr string
+  #[global]
+   Instance reprString : Repr string
     := {| repr s := ("" ++ show s ++ "")%string |}.
 
   Definition repr_raw_id (rid : raw_id) : string
@@ -59,7 +57,8 @@ Section ReprInstances.
        | Raw i  => "(Raw " ++ repr i ++ ")"
        end.
 
-  Global Instance reprRawId : Repr raw_id
+  #[global]
+   Instance reprRawId : Repr raw_id
     := {| repr := repr_raw_id |}.
 
   Definition repr_ident (i : ident) : string
@@ -68,54 +67,17 @@ Section ReprInstances.
        | ID_Local r  => "(ID_Local " ++ repr r ++ ")"
        end.
 
-  Global Instance reprIdent : Repr ident
+  #[global]
+   Instance reprIdent : Repr ident
     := {| repr := repr_ident |}.
 
-  Global Instance reprN : Repr N
+  #[global]
+   Instance reprN : Repr N
     := {| repr := show |}.
 
   Local Open Scope string.
 
-  Lemma contents_In {A : Type} (l : list A) (f : forall (x : A), In x l -> string) : string.
-  Proof.
-    induction l.
-    - exact "".
-    - destruct l.
-      + refine (f a _).
-        cbn. auto.
-      + refine ((f a _ ++ "; ") ++ @IHl _)%string.
-        * cbn. auto.
-        * intros x H.
-          apply (f x). cbn.
-          auto.
-  Defined.
-
-  (* I don't think I want to use sizeof_typ for measures... *)
-  (* TODO: Move this *)
-  Fixpoint typ_measure (t : typ) : nat :=
-    match t with
-    | TYPE_I sz => 0
-    | TYPE_IPTR => 0
-    | TYPE_Pointer t => S (typ_measure t)
-    | TYPE_Void => 0
-    | TYPE_Half => 0
-    | TYPE_Float => 0
-    | TYPE_Double => 0
-    | TYPE_X86_fp80 => 0
-    | TYPE_Fp128 => 0
-    | TYPE_Ppc_fp128 => 0
-    | TYPE_Metadata => 0
-    | TYPE_X86_mmx => 0
-    | TYPE_Array sz t => S (typ_measure t)
-    | TYPE_Function ret args _ => S (typ_measure ret + list_sum (map typ_measure args))
-    | TYPE_Struct fields => S (list_sum (map typ_measure fields))
-    | TYPE_Packed_struct fields => S (list_sum (map typ_measure fields))
-    | TYPE_Opaque => 0
-    | TYPE_Vector sz t => S (typ_measure t)
-    | TYPE_Identified id => 0
-    end.
-
-  Program Fixpoint repr_dtyp (t : dtyp) {measure (dtyp_measure t)} : string :=
+  Fixpoint repr_dtyp (t : dtyp) : string :=
     match t with
     | DTYPE_I sz => "(DTYPE_I " ++ repr sz ++ ")"
     | DTYPE_IPTR => "DTYPE_IPTR"
@@ -130,27 +92,13 @@ Section ReprInstances.
     | DTYPE_Metadata => "DTYPE_Metadata"
     | DTYPE_X86_mmx => "DTYPE_X86_mmx"
     | DTYPE_Array sz t => "(DTYPE_Array (" ++ repr sz ++ ") (" ++ repr_dtyp t ++ "))"
-    | DTYPE_Struct fields => "(DTYPE_Struct [" ++ contents_In fields (fun fld HIn => repr_dtyp fld) ++ "])"
-    | DTYPE_Packed_struct fields => "(DTYPE_Packed_struct [" ++ contents_In fields (fun fld HIn => repr_dtyp fld) ++ "])"
+    | DTYPE_Struct fields => "(DTYPE_Struct [" ++ (contents id (List.map repr_dtyp fields)) ++ "])"
+    | DTYPE_Packed_struct fields => "(DTYPE_Packed_struct [" ++ (contents id (List.map repr_dtyp fields)) ++ "])"
     | DTYPE_Opaque => "DTYPE_Opaque"
     | DTYPE_Vector sz t => "(DTYPE_Vector (" ++ repr sz ++ ") (" ++ repr_dtyp t ++ ")"
     end.
-  Next Obligation.
-    cbn.
-    lia.
-  Qed.
-  Next Obligation.
-    cbn.
-    pose proof (list_sum_map dtyp_measure fld fields HIn).
-    lia.
-  Qed.
-  Next Obligation.
-    cbn.
-    pose proof (list_sum_map dtyp_measure fld fields HIn).
-    lia.
-  Qed.
 
-  Program Fixpoint repr_typ (t : typ) {measure (typ_measure t)} : string :=
+  Fixpoint repr_typ (t : typ) : string :=
     match t with
     | TYPE_I sz                 => "(TYPE_I " ++ repr sz ++ ")"
     | TYPE_IPTR                 => "TYPE_IPTR"
@@ -165,38 +113,19 @@ Section ReprInstances.
     | TYPE_Metadata             => "TYPE_Metadata"
     | TYPE_X86_mmx              => "TYPE_X86_mmx"
     | TYPE_Array sz t           => "(TYPE_Array (" ++ repr sz ++ ") (" ++ repr_typ t ++ "))"
-    | TYPE_Function ret args varargs    => "(TYPE_Function (" ++ repr_typ ret ++ ") [" ++ contents_In args (fun arg HIn => repr_typ arg) ++ "]" ++ if varargs then "true" else "false" ++ ")"
-    | TYPE_Struct fields        => "(TYPE_Struct [" ++ contents_In fields (fun fld HIn => repr_typ fld) ++ "])"
-    | TYPE_Packed_struct fields => "(TYPE_Packed_struct [" ++ contents_In fields (fun fld HIn => repr_typ fld) ++ "])"
+    | TYPE_Function ret args varargs
+      => "(TYPE_Function (" ++ repr_typ ret ++ ") 
+        [" ++ (contents id (List.map repr_typ args)) ++ "]"
+        ++ if varargs then "true" else "false" ++ ")"
+    | TYPE_Struct fields        => "(TYPE_Struct [" ++ (contents id (List.map repr_typ fields)) ++ "])"
+    | TYPE_Packed_struct fields => "(TYPE_Packed_struct [" ++ (contents id (List.map repr_typ fields)) ++ "])"
     | TYPE_Opaque               => "TYPE_Opaque"
     | TYPE_Vector sz t          => "(TYPE_Vector (" ++ repr sz ++ ") (" ++ repr_typ t ++ ")"
     | TYPE_Identified id        => "(TYPE_Identified " ++ repr id ++ ")"
     end.
-  Next Obligation.
-    cbn in *.
-    lia.
-  Qed.
-  Next Obligation.
-    cbn in *.
-    lia.
-  Qed.
-  Next Obligation.
-    cbn.
-    pose proof (list_sum_map typ_measure arg args HIn).
-    lia.
-  Qed.
-  Next Obligation.
-    cbn.
-    pose proof (list_sum_map typ_measure fld fields HIn).
-    lia.
-  Qed.
-  Next Obligation.
-    cbn.
-    pose proof (list_sum_map typ_measure fld fields HIn).
-    lia.
-  Qed.
 
-  Global Instance reprTyp:  Repr typ :=
+  #[global]
+   Instance reprTyp:  Repr typ :=
     {|
     repr := repr_typ
     |}.
@@ -219,7 +148,8 @@ Section ReprInstances.
        | Xor     => "Xor"
        end.
 
-  Global Instance reprIBinop : Repr ibinop
+  #[global]
+   Instance reprIBinop : Repr ibinop
     := {| repr := repr_ibinop |}.
 
   Definition repr_icmp (cmp : icmp) : string
@@ -236,10 +166,12 @@ Section ReprInstances.
        | Sle => "Sle"
        end.
 
-  Global Instance reprICmp : Repr icmp
+  #[global]
+   Instance reprICmp : Repr icmp
     := {| repr := repr_icmp |}.
 
-  Global Instance reprPair (A B : Type) `{Repr A} `{Repr B} : Repr (A * B) :=
+  #[global]
+   Instance reprPair (A B : Type) `{Repr A} `{Repr B} : Repr (A * B) :=
     {|
     repr p :=
       match p with
@@ -247,84 +179,140 @@ Section ReprInstances.
       end
     |}.
 
-  (* Move this *)
-  Fixpoint exp_measure {T : Set} (e : exp T) : nat :=
-    match e with
-    | EXP_Ident id => 0
-    | EXP_Integer x => 0
-    | EXP_Float f => 0
-    | EXP_Double f => 0
-    | EXP_Hex f => 0
-    | EXP_Bool b => 0
-    | EXP_Null => 0
-    | EXP_Zero_initializer => 0
-    | EXP_Cstring elts => S (list_sum (map (fun et => exp_measure (snd et)) elts))
-    | EXP_Undef => 0
-    | EXP_Struct fields => S (list_sum (map (fun et => exp_measure (snd et)) fields))
-    | EXP_Packed_struct fields => S (list_sum (map (fun et => exp_measure (snd et)) fields))
-    | EXP_Array elts => S (list_sum (map (fun et => exp_measure (snd et)) elts))
-    | EXP_Vector elts => S (list_sum (map (fun et => exp_measure (snd et)) elts))
-    | OP_IBinop iop t v1 v2 => S (exp_measure v1 + exp_measure v2)
-    | OP_ICmp cmp t v1 v2 => S (exp_measure v1 + exp_measure v2)
-    | OP_FBinop fop fm t v1 v2 => S (exp_measure v1 + exp_measure v2)
-    | OP_FCmp cmp t v1 v2 => S (exp_measure v1 + exp_measure v2)
-    | OP_Conversion conv t_from v t_to => S (exp_measure v)
-    | OP_GetElementPtr t ptrval idxs => S (exp_measure (snd ptrval) + list_sum (map (fun et => exp_measure (snd et)) idxs))
-    | OP_ExtractElement vec idx => S (exp_measure (snd vec) + exp_measure (snd idx))
-    | OP_InsertElement vec elt idx => S (exp_measure (snd vec) + exp_measure (snd elt) + exp_measure (snd idx))
-    | OP_ShuffleVector vec1 vec2 idxmask => S (exp_measure (snd vec1) + exp_measure (snd vec2) + exp_measure (snd idxmask))
-    | OP_ExtractValue vec idxs => S (exp_measure (snd vec))
-    | OP_InsertValue vec elt idxs => S (exp_measure (snd vec) + exp_measure (snd elt))
-    | OP_Select cnd v1 v2 => S (exp_measure (snd cnd) + exp_measure (snd v1) + exp_measure (snd v2) )
-    | OP_Freeze v => S (exp_measure (snd v))
-    end.
-
   Definition pair_repr {A B : Type} (fa : A -> string) (fb : B -> string) (ab : A * B) : string :=
     match ab with
     | (a, b) =>
       "(" ++ fa a ++ ", " ++ fb b ++ ")"
     end.
 
+  Definition repr_conversion_type (c:conversion_type) : string :=
+    match c with 
+    | Trunc => "Trunc"
+    | Zext => "Zext"
+    | Sext => "Sext"
+    | Fptrunc => "Fptrunc"
+    | Fpext => "Fpext"
+    | Uitofp => "Uitofp"
+    | Sitofp => "Sitofp"
+    | Fptoui => "Fptoui"
+    | Fptosi => "Fptosi"
+    | Inttoptr  => "Inttoptr "
+    | Ptrtoint => "Ptrtoint"
+    | Bitcast => "Bitcast"
+    | Addrspacecast => "Addrspacecast"
+    end.
 
-  Ltac exp_measure_solve :=
-    solve [cbn; lia
-          |
-          cbn;
-          match goal with
-          | HIn : In ?x ?xs |- context [ list_sum (map ?f _)] =>
-            pose proof (list_sum_map f x xs HIn)
-          end;
-          cbn in *; lia
-          | repeat split; discriminate
-          ].
+  #[global]
+   Instance reprConversionType : Repr conversion_type :=
+    {| repr := repr_conversion_type |}.
 
-  Obligation Tactic := try Tactics.program_simpl; try solve [exp_measure_solve].
-  Program Fixpoint repr_exp (v : exp typ) {measure (exp_measure v)} : string :=
+  Definition repr_fbinop (f:fbinop) : string :=
+    match f with
+    | FAdd => "FAdd"
+    | FSub => "FSub"
+    | FMul => "FMul"
+    | FDiv => "FDiv"
+    | FRem => "FRem"
+    end.
+
+  #[global]
+   Instance reprFBinop : Repr fbinop :=
+    {| repr := repr_fbinop |}.
+  
+  Definition repr_fast_math (fm:fast_math) : string :=
+    match fm with
+    | Nnan => "Nnan"
+    | Ninf => "Ninf"
+    | Nsz => "Nsz"
+    | Arcp => "Arcp"
+    | Fast => "Fast"
+    end.
+
+  #[global]
+   Instance reprFastMath : Repr fast_math :=
+    {| repr := repr_fast_math |}.
+
+  Definition repr_fcmp (f:fcmp) : string :=
+    match f with
+    | FFalse => "FFalse"
+    | FOeq => "FOeq"
+    | FOgt => "FOgt"
+    | FOge => "FOge"
+    | FOlt => "FOlt"
+    | FOle => "FOle"
+    | FOne => "FOne"
+    | FOrd => "FOrd"
+    | FUno => "FUno"
+    | FUeq => "FUeq"
+    | FUgt => "FUgt"
+    | FUge => "FUge"
+    | FUlt => "FUlt"
+    | FUle => "FUle"
+    | FUne => "FUne"
+    | FTrue => "FTrue"
+    end.
+
+  #[global]
+   Instance reprFCmp : Repr fcmp :=
+    {| repr := repr_fcmp |}.
+  
+  Fixpoint repr_exp (v : exp typ) : string :=
+    let texp (te : (typ * exp typ)) : string :=
+      let '(t, e) := te in "(" ++ repr_typ t ++ ", " ++ repr_exp e ++ ")"
+    in
     match v with
     | EXP_Ident id => "(EXP_Ident " ++ repr id ++ ")"
     | EXP_Integer x => "(EXP_Integer " ++ repr x ++ ")"
+    | EXP_Float f => "(EXP_Float " ++ show f ++ ")"
+    | EXP_Double f => "(EXP_Double " ++ show f ++ ")"
+    | EXP_Hex f => "(EXP_Hex " ++ show f ++ ")"
     | EXP_Bool b => "(EXP_Bool " ++ repr b ++ ")"
     | EXP_Null => "EXP_Null"
     | EXP_Zero_initializer => "EXP_Zero_initializer"
-    | EXP_Cstring s =>
-      "(EXP_Cstring [" ++ contents_In s (fun '(t, e) HIn => "(" ++ repr t ++ ", " ++ repr_exp e ++ ")") ++ "])"
+    | EXP_Cstring s => "(EXP_Cstring [" ++ (contents id (List.map texp s)) ++ "])"
     | EXP_Undef => "EXP_Undef"
+    | EXP_Struct fields => "(EXP_Struct [" ++ (contents id (List.map texp fields)) ++ "])"
+    | EXP_Packed_struct fields => "(EXP_Packed_struct [" ++ (contents id (List.map texp fields)) ++ "])"
+    | EXP_Array fields => "(EXP_Array [" ++ (contents id (List.map texp fields)) ++ "])"
+    | EXP_Vector fields => "(EXP_vector [" ++ (contents id (List.map texp fields)) ++ "])"
     | OP_IBinop iop t v1 v2 =>
       "(OP_IBinop " ++ repr iop ++ " " ++ repr t ++ " " ++ repr_exp v1 ++ " " ++ repr_exp v2 ++ ")"
     | OP_ICmp cmp t v1 v2 =>
-      "(OP_ICmp " ++ repr cmp ++ " " ++ repr t ++ " " ++ repr_exp v1 ++ " " ++ repr_exp v2 ++ ")"
+        "(OP_ICmp " ++ repr cmp ++ " " ++ repr t ++ " " ++ repr_exp v1 ++ " " ++ repr_exp v2 ++ ")"
+    | OP_FBinop fop fm t v1 v2 =>
+        "(OP_FBinop " ++ repr fop ++ " [" ++ (contents id (List.map repr_fast_math fm)) ++
+                      "] " ++ repr t ++ " " ++ repr_exp v1 ++ " " ++ repr_exp v2 ++ ")"
+    | OP_FCmp cmp t v1 v2 =>
+        "(OP_FCmp " ++ repr cmp ++ " " ++ repr t ++ " " ++ repr_exp v1 ++ " " ++ repr_exp v2 ++ ")"
+    | OP_Conversion c from v to =>
+        "(OP_Conversion " ++ repr c ++ " " ++ repr from ++ " " ++ repr_exp v ++ " " ++ repr to ++ ")"
     | OP_GetElementPtr t ptrval idxs =>
-      "(OP_GetElementPtr " ++ repr t ++
-                           "(" ++ repr (fst ptrval) ++ ", " ++ repr_exp (snd ptrval) ++ ") [" ++ contents_In idxs (fun '(t, e) Hin => "(" ++ repr t ++ ", " ++ repr_exp e ++ ")") ++ "])"
-    | OP_Select (tc, cnd) (t1, v1) (t2, v2) =>
-      "(OP_Select ( " ++ repr tc ++ ", " ++ repr_exp cnd ++ ") (" ++ repr t1 ++ ", " ++ repr_exp v1  ++ ") (" ++ repr t2 ++ ", " ++ repr_exp v2 ++ "))"
-    | _ => "repr_exp todo"
+        "(OP_GetElementPtr " ++ repr t ++
+                             "(" ++ texp ptrval ++  ") ["
+                             ++ (contents id (List.map texp idxs)) ++ "])"
+    | OP_ExtractElement v i =>
+        "(OP_ExtractElement " ++ texp v ++ " " ++ texp i ++ ")"
+    | OP_InsertElement v e i =>
+        "(OP_ExtractElement " ++ texp v ++ " " ++ texp e ++ " " ++ texp i ++ ")"
+    | OP_ShuffleVector v1 v2 mask =>
+        "(OP_ShuffleVector " ++ texp v1 ++ " " ++ texp v2 ++ " " ++ texp mask ++ ")"
+    | OP_ExtractValue v idxs =>
+        "(OP_ExtractValue " ++ texp v ++ " [" ++ (contents id (List.map show idxs)) ++ "])"
+    | OP_InsertValue v e idxs =>
+        "(OP_ExtractValue " ++ texp v ++ " " ++ texp e ++ " [" ++ (contents id (List.map show idxs)) ++ "])"
+    | OP_Select cnd v1 v2 =>
+        "(OP_Select " ++ texp cnd ++ " " ++ texp v1 ++ " " ++ texp v2 ++ ")"
+    | OP_Freeze v =>
+        "(OP_Freez " ++ texp v ++")"
     end.
+                                          
 
-  Global Instance reprExp : Repr (exp typ)
+  #[global]
+   Instance reprExp : Repr (exp typ)
     := {| repr := repr_exp |}.
 
-  Global Instance reprTExp : Repr (texp typ)
+  #[global]
+   Instance reprTExp : Repr (texp typ)
     := {| repr te :=
             match te with
             | (t, e) => "(" ++ repr t ++ ", " ++ repr e ++ ")"
@@ -337,7 +325,8 @@ Section ReprInstances.
        | Some a => "(Some " ++ repr a ++ ")"
        end.
 
-  Global Instance reprOption (A : Type) `{Repr A} : Repr (option A) :=
+  #[global]
+   Instance reprOption (A : Type) `{Repr A} : Repr (option A) :=
     {| repr := repr_opt |}.
 
   Definition repr_instr (i : instr typ) : string
@@ -353,10 +342,12 @@ Section ReprInstances.
        | _ => "repr_instr todo"
        end.
 
-  Global Instance reprInstr : Repr (instr typ)
+  #[global]
+   Instance reprInstr : Repr (instr typ)
     := {| repr := repr_instr |}.
 
-  Global Instance reprInstrId : Repr instr_id
+  #[global]
+   Instance reprInstrId : Repr instr_id
     := {| repr i :=
             match i with
             | IId raw => ("(IId " ++ repr raw ++ ")")%string
@@ -374,7 +365,8 @@ Section ReprInstances.
        | _ => "repr_terminator todo"
        end.
 
-  Global Instance reprTerminator : Repr (terminator typ)
+  #[global]
+   Instance reprTerminator : Repr (terminator typ)
     := {| repr := repr_terminator |}.
 
   Definition repr_phi (p : phi typ) : string
@@ -383,7 +375,8 @@ Section ReprInstances.
          "(Phi " ++ repr t ++ repr args ++ ")"
        end.
 
-  Global Instance reprPhi : Repr (phi typ)
+  #[global]
+   Instance reprPhi : Repr (phi typ)
     := {| repr := repr_phi
        |}.
 
@@ -394,7 +387,8 @@ Section ReprInstances.
         "(mk_block " ++ repr blk_id ++ " " ++ repr blk_phis ++ " " ++ repr blk_code ++ " " ++ repr blk_term ++ " " ++ repr blk_comments ++ ")"
       end.
 
-  Global Instance reprBlock: Repr (block typ) :=
+  #[global]
+   Instance reprBlock: Repr (block typ) :=
     {|
     repr := repr_block
     |}.
@@ -430,7 +424,8 @@ Section ReprInstances.
     | PARAMATTR_Nofree => "PARAMATTR_Nofree"
     end.
 
-  Global Instance reprParamAttr : Repr (param_attr) :=
+  #[global]
+   Instance reprParamAttr : Repr (param_attr) :=
     {| repr := repr_param_attr |}.
 
   Definition repr_linkage (l : linkage) : string :=
@@ -448,7 +443,8 @@ Section ReprInstances.
     | LINKAGE_External => "LINKAGE_External"
     end.
 
-  Global Instance reprLinkage : Repr linkage :=
+  #[global]
+   Instance reprLinkage : Repr linkage :=
     {| repr := repr_linkage |}.
 
   Definition repr_visibility (v : visibility) : string :=
@@ -458,7 +454,8 @@ Section ReprInstances.
     | VISIBILITY_Protected => "VISIBILITY_Protected"
     end.
 
-  Global Instance reprVisibility : Repr visibility :=
+  #[global]
+   Instance reprVisibility : Repr visibility :=
     {| repr := repr_visibility |}.
 
   Definition repr_dll_storage (d : dll_storage) : string :=
@@ -467,7 +464,8 @@ Section ReprInstances.
     | DLLSTORAGE_Dllexport => "DLLSTORAGE_Dllexport"
     end.
 
-  Global Instance reprDll_Storage : Repr dll_storage :=
+  #[global]
+   Instance reprDll_Storage : Repr dll_storage :=
     {| repr := repr_dll_storage |}.
 
   Definition repr_cconv (c : cconv) : string :=
@@ -487,7 +485,8 @@ Section ReprInstances.
     | CC_Preserve_mostc => "CC_Preserve_mostc"                  
     end.
 
-  Global Instance reprCconv : Repr cconv :=
+  #[global]
+   Instance reprCconv : Repr cconv :=
     {| repr := repr_cconv |}.
 
   Definition repr_fn_attr (fa : fn_attr) : string :=
@@ -592,7 +591,8 @@ Section ReprInstances.
     | FNATTR_Attr_grp g => "(FNATTR_Attr_grp " ++ repr g ++ ")"
     end.
 
-  Global Instance reprFn_Attr : Repr fn_attr :=
+  #[global]
+   Instance reprFn_Attr : Repr fn_attr :=
     {| repr := repr_fn_attr |}.
 
   
@@ -603,41 +603,34 @@ Section ReprInstances.
     | TLS_Localexec => "TLS_Localexec"
     end.
   
-  Global Instance reprThread_Local_Storage : Repr thread_local_storage :=
+  #[global]
+   Instance reprThread_Local_Storage : Repr thread_local_storage :=
     {| repr := repr_thread_local_storage |}.
 
-  Fixpoint metadata_measure (m : metadata typ) : nat
-    := match m with
-       | METADATA_Const tv => 0
-       | METADATA_Null => 0
-       | METADATA_Id id => 0
-       | METADATA_String str => 0
-       | METADATA_Named strs => 0
-       | METADATA_Node mds => S (list_sum (map metadata_measure mds))
-       end.
-        
-  Program Fixpoint repr_metadata (m : metadata typ) {measure (metadata_measure m)}: string :=
+  Program Fixpoint repr_metadata (m : metadata typ) : string :=
     match m with
     | METADATA_Const tv => "(METADATA_Const " ++ repr tv ++ ")"
     | METADATA_Null => "METADATA_Null"
     | METADATA_Id id => "(METADATA_Id " ++ repr id ++ ")"
     | METADATA_String str => "(METADATA_String " ++ repr str ++ ")"
     | METADATA_Named strs => "(METADATA_Named " ++ repr strs ++ ")"
-    | METADATA_Node mds => "(METADATA_Node [" ++ contents_In mds (fun md Hin => repr_metadata md) ++ "])"
+    | METADATA_Node mds => "(METADATA_Node [" ++ (contents id (List.map repr_metadata mds)) ++ "])"
     end.
 
-  Global Instance reprMetadata : Repr (metadata typ) :=
+  #[global]
+   Instance reprMetadata : Repr (metadata typ) :=
     {| repr := repr_metadata |}.
 
 
   Definition repr_preemption_specifier (p:preemption_specifier) : string :=
     match p with
-    | PREEMPTION_Dso_premptable => "PREEMPTION_Dso_premptable"
+    | PREEMPTION_Dso_preemptable => "PREEMPTION_Dso_preemptable"
     | PREEMPTION_Dso_local => "PREEMPTION_Dso_local"
     end
   .
 
-  Global Instance reprPremptionSpecifier : Repr (preemption_specifier) :=
+  #[global]
+   Instance reprPremptionSpecifier : Repr (preemption_specifier) :=
     {| repr := repr_preemption_specifier |}.
 
 
@@ -647,7 +640,8 @@ Section ReprInstances.
     | Local_Unnamed_addr => "Local_Unnamed_addr"
     end.
 
-  Global Instance reprUnnamedAddr : Repr (unnamed_addr) :=
+  #[global]
+   Instance reprUnnamedAddr : Repr (unnamed_addr) :=
     {| repr := repr_unnamed_addr |}.
   
   
@@ -676,33 +670,36 @@ Section ReprInstances.
     | ANN_personality t => "ANN_personality " ++ (repr t)
   end.
   
-  Global Instance reprAnnotation : Repr (annotation typ) :=
+  #[global]
+   Instance reprAnnotation : Repr (annotation typ) :=
     {| repr := repr_annotation |}.
   
   Definition repr_declaration (dec : declaration typ) : string
     := match dec with
-       | mk_declaration dc_name dc_type dc_param_attrs dc_attrs dc_annotations =>
+       | mk_declaration dc_name dc_type dc_param_attrs dc_annotations =>
          "(mk_declaration " ++ repr dc_name ++ " "
                             ++ repr dc_type ++ " "
                             ++ repr dc_param_attrs ++ " "
-                            ++ repr dc_attrs ++ " "
                             ++ repr dc_annotations
 
        end.
   
-  Global Instance reprDeclaration : Repr (declaration typ) :=
+  #[global]
+   Instance reprDeclaration : Repr (declaration typ) :=
     {| repr := repr_declaration |}.
 
   Definition repr_definition (defn : definition typ (block typ * list (block typ))) : string
     :=
       match defn with
-      | mk_definition _ df_prototype df_args df_instrs =>
+      | mk_definition df_prototype df_args df_attrs df_instrs =>
         "(mk_definition _ " ++ repr df_prototype ++ " "
-                          ++ repr df_args ++ " "
-                          ++ repr df_instrs ++ ")"
+                            ++ repr df_args ++ " "
+                            ++ repr df_attrs ++ " "
+                            ++ repr df_instrs ++ ")"
       end.
 
-  Global Instance reprDefinition: Repr (definition typ (block typ * list (block typ))) :=
+  #[global]
+   Instance reprDefinition: Repr (definition typ (block typ * list (block typ))) :=
     {| repr := repr_definition |}.
 
   Definition repr_global (g : global typ) : string :=
@@ -717,7 +714,8 @@ Section ReprInstances.
                     ++ ")"
     end.
 
-  Global Instance reprGlobal : Repr (global typ) :=
+  #[global]
+   Instance reprGlobal : Repr (global typ) :=
     {| repr := repr_global |}.
 
 
@@ -735,7 +733,8 @@ Section ReprInstances.
        | TLE_Attribute_group i attrs => "(TLE_Attribute_group " ++ repr i ++ " " ++ repr attrs ++ ")"
        end.
 
-  Global Instance reprTLE: Repr (toplevel_entity typ (block typ * list (block typ))) :=
+  #[global]
+   Instance reprTLE: Repr (toplevel_entity typ (block typ * list (block typ))) :=
     {| repr := repr_tle |}.
 
 End ReprInstances.
