src/coq/Syntax/Traversal.v
@@ -285,7 +285,6 @@ Section Endo.
            `{Endo string}
            `{Endo int}
            `{Endo param_attr}
-           `{Endo fn_attr}
            `{Endo (annotation T)}
            `{Endo (exp T)}
       : Endo (declaration T) | 50 :=
@@ -293,7 +292,6 @@ Section Endo.
               (endo (dc_name d))
               (endo (dc_type d))
               (endo (dc_param_attrs d))
-              (endo (dc_attrs d))
               (endo (dc_annotations d))
     .
 
@@ -301,12 +299,14 @@ Section Endo.
            {FnBody:Set}
            `{Endo (declaration T)}
            `{Endo raw_id}
+           `{Endo fn_attr}
            `{Endo FnBody}
       : Endo (definition T FnBody) | 50 :=
       fun d =>
         mk_definition _
                       (endo (df_prototype d))
                       (endo (df_args d))
+                      (endo (df_attrs d))
                       (endo (df_instrs d)).
 
     #[global] Instance Endo_toplevel_entity
@@ -343,6 +343,7 @@ Section Endo.
            `{Endo T}
            `{Endo (global T)}
            `{Endo (declaration T)}
+           `{Endo fn_attr}
            `{Endo raw_id}
       : Endo (modul FnBody) | 50 :=
       fun m =>
@@ -614,6 +615,7 @@ Section TFunctor.
     (* SAZ: Not as parameterized as it could be - how often do we want to change annnotations? *)
     #[global] Instance TFunctor_annotation
      `{TFunctor exp}
+     `{Endo raw_id}
      `{TFunctor metadata}
       : TFunctor annotation | 50 :=
       fun U V f a =>
@@ -633,7 +635,7 @@ Section TFunctor.
         | ANN_no_sanitize_address => ANN_no_sanitize_address
         | ANN_no_sanitize_hwaddress => ANN_no_sanitize_hwaddress
         | ANN_sanitize_address_dyninit => ANN_sanitize_address_dyninit
-        | ANN_metadata l => ANN_metadata (tfmap f l)
+        | ANN_metadata l => ANN_metadata (tfmap (fun '(x,y) => (endo x, tfmap f y)) l)
         | ANN_cconv c => ANN_cconv c
         | ANN_gc s => ANN_gc s
         | ANN_prefix t => ANN_prefix (tfmap f t)
@@ -668,7 +670,6 @@ Section TFunctor.
            `{Endo visibility}
            `{Endo dll_storage}
            `{Endo cconv}
-           `{Endo fn_attr}
            `{TFunctor exp}
            `{TFunctor metadata}
       : TFunctor declaration | 50 :=
@@ -676,7 +677,6 @@ Section TFunctor.
                        (endo (dc_name d))
                        (f (dc_type d))
                        (endo (dc_param_attrs d))
-                       (endo (dc_attrs d))
                        (tfmap f (dc_annotations d))
           .
 
@@ -685,12 +685,14 @@ Section TFunctor.
            {FnBody:Set -> Set}
            `{TFunctor declaration}
            `{Endo raw_id}
+           `{Endo fn_attr}
            `{TFunctor FnBody}
       : TFunctor (fun T => definition T (FnBody T)) | 50 :=
       fun U V f d =>
         mk_definition _
                       (tfmap f (df_prototype d))
                       (endo (df_args d))
+                      (endo (df_attrs d))
                       (tfmap f (df_instrs d)).
 
     #[global] Instance TFunctor_toplevel_entity
@@ -830,7 +832,7 @@ Section Examples.
     Instance subst_cfg_endo_cfg: Endo (definition T (cfg T)) :=
       fun f =>
         if (dc_name (df_prototype f)) ~=? fid
-        then {| df_prototype := df_prototype f; df_args := df_args f ; df_instrs := new_f |}
+        then {| df_prototype := df_prototype f; df_args := df_args f ; df_attrs := df_attrs f ; df_instrs := new_f |}
         else f.
 
     Definition subst_cfg: Endo (mcfg T) := endo.
